proofs start

lib/libcoq.ml
@@ -1,622 +1,604 @@
+
 (** val add : int -> int -> int **)
 
-let add = ( + )
+let rec add = (+)
 
-(** val sub : int -> int -> int **)
-
-let sub = fun n m -> Stdlib.max 0 (n - m)
-
-module Nat = struct
+module Nat =
+ struct
   (** val ltb : int -> int -> bool **)
 
-  let ltb n m = Stdlib.Int.succ n <= m
-end
+  let ltb n m =
+    (<=) (Stdlib.Int.succ n) m
+ end
 
-module Red_black_tree = struct
+module Red_black_tree =
+ struct
   type key = int
-  type color = Red | Black
+
+  type color =
+  | Red
+  | Black
 
   (** val color_rect : 'a1 -> 'a1 -> color -> 'a1 **)
 
-  let color_rect f f0 = function Red -> f | Black -> f0
+  let color_rect f f0 = function
+  | Red -> f
+  | Black -> f0
 
   (** val color_rec : 'a1 -> 'a1 -> color -> 'a1 **)
 
-  let color_rec f f0 = function Red -> f | Black -> f0
+  let color_rec f f0 = function
+  | Red -> f
+  | Black -> f0
 
   type 'v rbtree =
-    | Coq_nil
-    | Coq_node of color * 'v rbtree * key * 'v * 'v rbtree
+  | Coq_nil
+  | Coq_node of color * 'v rbtree * key * 'v * 'v rbtree
 
-  (** val rbtree_rect : 'a2 -> (color -> 'a1 rbtree -> 'a2 -> key -> 'a1 -> 'a1
-      rbtree -> 'a2 -> 'a2) -> 'a1 rbtree -> 'a2 **)
+  (** val rbtree_rect :
+      'a2 -> (color -> 'a1 rbtree -> 'a2 -> key -> 'a1 -> 'a1 rbtree -> 'a2
+      -> 'a2) -> 'a1 rbtree -> 'a2 **)
 
   let rec rbtree_rect f f0 = function
-    | Coq_nil -> f
-    | Coq_node (c, r0, k, y, r1) ->
-        f0 c r0 (rbtree_rect f f0 r0) k y r1 (rbtree_rect f f0 r1)
+  | Coq_nil -> f
+  | Coq_node (c, r0, k, y, r1) ->
+    f0 c r0 (rbtree_rect f f0 r0) k y r1 (rbtree_rect f f0 r1)
 
-  (** val rbtree_rec : 'a2 -> (color -> 'a1 rbtree -> 'a2 -> key -> 'a1 -> 'a1
-      rbtree -> 'a2 -> 'a2) -> 'a1 rbtree -> 'a2 **)
+  (** val rbtree_rec :
+      'a2 -> (color -> 'a1 rbtree -> 'a2 -> key -> 'a1 -> 'a1 rbtree -> 'a2
+      -> 'a2) -> 'a1 rbtree -> 'a2 **)
 
   let rec rbtree_rec f f0 = function
-    | Coq_nil -> f
-    | Coq_node (c, r0, k, y, r1) ->
-        f0 c r0 (rbtree_rec f f0 r0) k y r1 (rbtree_rec f f0 r1)
+  | Coq_nil -> f
+  | Coq_node (c, r0, k, y, r1) ->
+    f0 c r0 (rbtree_rec f f0 r0) k y r1 (rbtree_rec f f0 r1)
 
   (** val mk_nil : 'a1 rbtree **)
 
-  let mk_nil = Coq_nil
+  let mk_nil =
+    Coq_nil
 
   (** val lookup : key -> 'a1 rbtree -> 'a1 option **)
 
   let rec lookup x = function
-    | Coq_nil -> None
-    | Coq_node (_, l, k, v, r) ->
-        if x < k then lookup x l else if k < x then lookup x r else Some v
+  | Coq_nil -> None
+  | Coq_node (_, l, k, v, r) ->
+    if ( < ) x k then lookup x l else if ( < ) k x then lookup x r else Some v
 
   (** val max : 'a1 rbtree -> (key * 'a1) option **)
 
   let rec max = function
-    | Coq_nil -> None
-    | Coq_node (_, _, k, vk, r) -> (
-        match r with
-        | Coq_nil -> Some (k, vk)
-        | Coq_node (_, _, _, _, _) -> max r)
+  | Coq_nil -> None
+  | Coq_node (_, _, k, vk, r) ->
+    (match r with
+     | Coq_nil -> Some (k , vk)
+     | Coq_node (_, _, _, _, _) -> max r)
 
   (** val min : 'a1 rbtree -> (key * 'a1) option **)
 
   let rec min = function
-    | Coq_nil -> None
-    | Coq_node (_, l, k, vk, _) -> (
-        match l with
-        | Coq_nil -> Some (k, vk)
-        | Coq_node (_, _, _, _, _) -> min l)
+  | Coq_nil -> None
+  | Coq_node (_, l, k, vk, _) ->
+    (match l with
+     | Coq_nil -> Some (k , vk)
+     | Coq_node (_, _, _, _, _) -> min l)
 
-  module BalanceDetails = struct
-    (** val rot_left : 'a1 rbtree -> 'a1 rbtree **)
+  (** val rot_left : 'a1 rbtree -> 'a1 rbtree **)
 
-    let rot_left = function
-      | Coq_nil -> Coq_nil
-      | Coq_node (tc, a, k, v, t_r) -> (
-          match t_r with
-          | Coq_nil -> Coq_node (tc, a, k, v, t_r)
-          | Coq_node (rc, b, rk, rv, c) ->
-              Coq_node (rc, Coq_node (Red, a, k, v, b), rk, rv, c))
+  let rot_left = function
+  | Coq_nil -> Coq_nil
+  | Coq_node (tc, a, k, v, t_r) ->
+    (match t_r with
+     | Coq_nil -> Coq_node (tc, a, k, v, t_r)
+     | Coq_node (rc, b, rk, rv, c) ->
+       Coq_node (rc, (Coq_node (Red, a, k, v, b)), rk, rv, c))
 
-    (** val rot_right : 'a1 rbtree -> 'a1 rbtree **)
+  (** val rot_right : 'a1 rbtree -> 'a1 rbtree **)
 
-    let rot_right = function
-      | Coq_nil -> Coq_nil
-      | Coq_node (tc, t_l, k, v, c) -> (
-          match t_l with
-          | Coq_nil -> Coq_node (tc, t_l, k, v, c)
-          | Coq_node (lc, a, lk, lv, b) ->
-              Coq_node (lc, a, lk, lv, Coq_node (Red, b, k, v, c)))
+  let rot_right = function
+  | Coq_nil -> Coq_nil
+  | Coq_node (tc, t_l, k, v, c) ->
+    (match t_l with
+     | Coq_nil -> Coq_node (tc, t_l, k, v, c)
+     | Coq_node (lc, a, lk, lv, b) ->
+       Coq_node (lc, a, lk, lv, (Coq_node (Red, b, k, v, c))))
 
-    (** val flip_colors : 'a1 rbtree -> 'a1 rbtree **)
+  (** val flip_colors : 'a1 rbtree -> 'a1 rbtree **)
 
-    let flip_colors t =
-      match t with
-      | Coq_nil -> t
-      | Coq_node (c, r, k, v, r0) -> (
-          match c with
-          | Red -> t
-          | Black -> (
-              match r with
+  let flip_colors t = match t with
+  | Coq_nil -> t
+  | Coq_node (c, r, k, v, r0) ->
+    (match c with
+     | Red -> t
+     | Black ->
+       (match r with
+        | Coq_nil -> t
+        | Coq_node (c0, ll, lk, lv, lr) ->
+          (match c0 with
+           | Red ->
+             (match r0 with
               | Coq_nil -> t
-              | Coq_node (c0, ll, lk, lv, lr) -> (
-                  match c0 with
-                  | Red -> (
-                      match r0 with
-                      | Coq_nil -> t
-                      | Coq_node (c1, rl, rk, rv, rr) -> (
-                          match c1 with
+              | Coq_node (c1, rl, rk, rv, rr) ->
+                (match c1 with
+                 | Red ->
+                   Coq_node (Red, (Coq_node (Black, ll, lk, lv, lr)), k, v,
+                     (Coq_node (Black, rl, rk, rv, rr)))
+                 | Black -> t))
+           | Black -> t)))
+
+  (** val make_black : 'a1 rbtree -> 'a1 rbtree **)
+
+  let make_black = function
+  | Coq_nil -> Coq_nil
+  | Coq_node (_, a, x, vx, b) -> Coq_node (Black, a, x, vx, b)
+
+  (** val balance : 'a1 rbtree -> 'a1 rbtree **)
+
+  let balance = function
+  | Coq_nil -> Coq_nil
+  | Coq_node (c, l, k, vk, r) ->
+    (match c with
+     | Red -> Coq_node (Red, l, k, vk, r)
+     | Black ->
+       (match l with
+        | Coq_nil ->
+          (match r with
+           | Coq_nil -> Coq_node (Black, l, k, vk, r)
+           | Coq_node (c0, b, y, vy, d) ->
+             (match c0 with
+              | Red ->
+                (match b with
+                 | Coq_nil ->
+                   (match d with
+                    | Coq_nil -> Coq_node (Black, l, k, vk, r)
+                    | Coq_node (c1, c2, z, vz, d0) ->
+                      (match c1 with
+                       | Red ->
+                         Coq_node (Red, (Coq_node (Black, l, k, vk, b)), y,
+                           vy, (Coq_node (Black, c2, z, vz, d0)))
+                       | Black -> Coq_node (Black, l, k, vk, r)))
+                 | Coq_node (c1, b0, y0, vy0, c2) ->
+                   (match c1 with
+                    | Red ->
+                      Coq_node (Red, (Coq_node (Black, l, k, vk, b0)), y0,
+                        vy0, (Coq_node (Black, c2, y, vy, d)))
+                    | Black ->
+                      (match d with
+                       | Coq_nil -> Coq_node (Black, l, k, vk, r)
+                       | Coq_node (c3, c4, z, vz, d0) ->
+                         (match c3 with
                           | Red ->
-                              Coq_node
-                                ( Red,
-                                  Coq_node (Black, ll, lk, lv, lr),
-                                  k,
-                                  v,
-                                  Coq_node (Black, rl, rk, rv, rr) )
-                          | Black -> t))
-                  | Black -> t)))
-
-    (** val make_black : 'a1 rbtree -> 'a1 rbtree **)
-
-    let make_black = function
-      | Coq_nil -> Coq_nil
-      | Coq_node (_, a, x, vx, b) -> Coq_node (Black, a, x, vx, b)
-
-    (** val balance : 'a1 rbtree -> 'a1 rbtree **)
-
-    let balance t =
-      match t with
-      | Coq_nil -> Coq_nil
-      | Coq_node (c, l, k, vk, r) -> (
-          match c with
-          | Red -> t
-          | Black -> (
-              match l with
-              | Coq_nil -> (
-                  match r with
-                  | Coq_nil -> t
-                  | Coq_node (c0, r0, _, _, r1) -> (
-                      match c0 with
-                      | Red -> (
-                          match r0 with
-                          | Coq_nil -> (
-                              match r1 with
-                              | Coq_nil -> t
-                              | Coq_node (c1, _, _, _, _) -> (
-                                  match c1 with
-                                  | Red -> flip_colors (make_black (rot_left t))
-                                  | Black -> t))
-                          | Coq_node (c1, _, _, _, _) -> (
-                              match c1 with
-                              | Red ->
-                                  let temp_t =
-                                    Coq_node (Black, l, k, vk, rot_right r)
-                                  in
-                                  flip_colors (make_black (rot_left temp_t))
-                              | Black -> (
-                                  match r1 with
-                                  | Coq_nil -> t
-                                  | Coq_node (c2, _, _, _, _) -> (
-                                      match c2 with
+                            Coq_node (Red, (Coq_node (Black, l, k, vk, b)),
+                              y, vy, (Coq_node (Black, c4, z, vz, d0)))
+                          | Black -> Coq_node (Black, l, k, vk, r)))))
+              | Black -> Coq_node (Black, l, k, vk, r)))
+        | Coq_node (c0, a, x, vx, c1) ->
+          (match c0 with
+           | Red ->
+             (match a with
+              | Coq_nil ->
+                (match c1 with
+                 | Coq_nil ->
+                   (match r with
+                    | Coq_nil -> Coq_node (Black, l, k, vk, r)
+                    | Coq_node (c2, b, y, vy, d) ->
+                      (match c2 with
+                       | Red ->
+                         (match b with
+                          | Coq_nil ->
+                            (match d with
+                             | Coq_nil -> Coq_node (Black, l, k, vk, r)
+                             | Coq_node (c3, c4, z, vz, d0) ->
+                               (match c3 with
+                                | Red ->
+                                  Coq_node (Red, (Coq_node (Black, l, k, vk,
+                                    b)), y, vy, (Coq_node (Black, c4, z, vz,
+                                    d0)))
+                                | Black -> Coq_node (Black, l, k, vk, r)))
+                          | Coq_node (c3, b0, y0, vy0, c4) ->
+                            (match c3 with
+                             | Red ->
+                               Coq_node (Red, (Coq_node (Black, l, k, vk,
+                                 b0)), y0, vy0, (Coq_node (Black, c4, y, vy,
+                                 d)))
+                             | Black ->
+                               (match d with
+                                | Coq_nil -> Coq_node (Black, l, k, vk, r)
+                                | Coq_node (c5, c6, z, vz, d0) ->
+                                  (match c5 with
+                                   | Red ->
+                                     Coq_node (Red, (Coq_node (Black, l, k,
+                                       vk, b)), y, vy, (Coq_node (Black, c6,
+                                       z, vz, d0)))
+                                   | Black -> Coq_node (Black, l, k, vk, r)))))
+                       | Black -> Coq_node (Black, l, k, vk, r)))
+                 | Coq_node (c2, b, y, vy, c3) ->
+                   (match c2 with
+                    | Red ->
+                      Coq_node (Red, (Coq_node (Black, a, x, vx, b)), y, vy,
+                        (Coq_node (Black, c3, k, vk, r)))
+                    | Black ->
+                      (match r with
+                       | Coq_nil -> Coq_node (Black, l, k, vk, r)
+                       | Coq_node (c4, b0, y0, vy0, d) ->
+                         (match c4 with
+                          | Red ->
+                            (match b0 with
+                             | Coq_nil ->
+                               (match d with
+                                | Coq_nil -> Coq_node (Black, l, k, vk, r)
+                                | Coq_node (c5, c6, z, vz, d0) ->
+                                  (match c5 with
+                                   | Red ->
+                                     Coq_node (Red, (Coq_node (Black, l, k,
+                                       vk, b0)), y0, vy0, (Coq_node (Black,
+                                       c6, z, vz, d0)))
+                                   | Black -> Coq_node (Black, l, k, vk, r)))
+                             | Coq_node (c5, b1, y1, vy1, c6) ->
+                               (match c5 with
+                                | Red ->
+                                  Coq_node (Red, (Coq_node (Black, l, k, vk,
+                                    b1)), y1, vy1, (Coq_node (Black, c6, y0,
+                                    vy0, d)))
+                                | Black ->
+                                  (match d with
+                                   | Coq_nil -> Coq_node (Black, l, k, vk, r)
+                                   | Coq_node (c7, c8, z, vz, d0) ->
+                                     (match c7 with
                                       | Red ->
-                                          flip_colors (make_black (rot_left t))
-                                      | Black -> t))))
-                      | Black -> t))
-              | Coq_node (c0, r0, _, _, r1) -> (
-                  match c0 with
-                  | Red -> (
-                      match r0 with
-                      | Coq_nil -> (
-                          match r1 with
-                          | Coq_nil -> (
-                              match r with
-                              | Coq_nil -> t
-                              | Coq_node (c1, r2, _, _, r3) -> (
-                                  match c1 with
-                                  | Red -> (
-                                      match r2 with
-                                      | Coq_nil -> (
-                                          match r3 with
-                                          | Coq_nil -> t
-                                          | Coq_node (c2, _, _, _, _) -> (
-                                              match c2 with
-                                              | Red ->
-                                                  flip_colors
-                                                    (make_black (rot_left t))
-                                              | Black -> t))
-                                      | Coq_node (c2, _, _, _, _) -> (
-                                          match c2 with
-                                          | Red ->
-                                              let temp_t =
-                                                Coq_node
-                                                  (Black, l, k, vk, rot_right r)
-                                              in
-                                              flip_colors
-                                                (make_black (rot_left temp_t))
-                                          | Black -> (
-                                              match r3 with
-                                              | Coq_nil -> t
-                                              | Coq_node (c3, _, _, _, _) -> (
-                                                  match c3 with
-                                                  | Red ->
-                                                      flip_colors
-                                                        (make_black (rot_left t))
-                                                  | Black -> t))))
-                                  | Black -> t))
-                          | Coq_node (c1, _, _, _, _) -> (
-                              match c1 with
-                              | Red ->
-                                  let temp_t =
-                                    Coq_node (Black, rot_left l, k, vk, r)
-                                  in
-                                  flip_colors (make_black (rot_right temp_t))
-                              | Black -> (
-                                  match r with
-                                  | Coq_nil -> t
-                                  | Coq_node (c2, r2, _, _, r3) -> (
-                                      match c2 with
-                                      | Red -> (
-                                          match r2 with
-                                          | Coq_nil -> (
-                                              match r3 with
-                                              | Coq_nil -> t
-                                              | Coq_node (c3, _, _, _, _) -> (
-                                                  match c3 with
-                                                  | Red ->
-                                                      flip_colors
-                                                        (make_black (rot_left t))
-                                                  | Black -> t))
-                                          | Coq_node (c3, _, _, _, _) -> (
-                                              match c3 with
-                                              | Red ->
-                                                  let temp_t =
-                                                    Coq_node
-                                                      ( Black,
-                                                        l,
-                                                        k,
-                                                        vk,
-                                                        rot_right r )
-                                                  in
-                                                  flip_colors
-                                                    (make_black
-                                                       (rot_left temp_t))
-                                              | Black -> (
-                                                  match r3 with
-                                                  | Coq_nil -> t
-                                                  | Coq_node (c4, _, _, _, _)
-                                                    -> (
-                                                      match c4 with
-                                                      | Red ->
-                                                          flip_colors
-                                                            (make_black
-                                                               (rot_left t))
-                                                      | Black -> t))))
-                                      | Black -> t))))
-                      | Coq_node (c1, _, _, _, _) -> (
-                          match c1 with
-                          | Red -> flip_colors (make_black (rot_right t))
-                          | Black -> (
-                              match r1 with
-                              | Coq_nil -> (
-                                  match r with
-                                  | Coq_nil -> t
-                                  | Coq_node (c2, r2, _, _, r3) -> (
-                                      match c2 with
-                                      | Red -> (
-                                          match r2 with
-                                          | Coq_nil -> (
-                                              match r3 with
-                                              | Coq_nil -> t
-                                              | Coq_node (c3, _, _, _, _) -> (
-                                                  match c3 with
-                                                  | Red ->
-                                                      flip_colors
-                                                        (make_black (rot_left t))
-                                                  | Black -> t))
-                                          | Coq_node (c3, _, _, _, _) -> (
-                                              match c3 with
-                                              | Red ->
-                                                  let temp_t =
-                                                    Coq_node
-                                                      ( Black,
-                                                        l,
-                                                        k,
-                                                        vk,
-                                                        rot_right r )
-                                                  in
-                                                  flip_colors
-                                                    (make_black
-                                                       (rot_left temp_t))
-                                              | Black -> (
-                                                  match r3 with
-                                                  | Coq_nil -> t
-                                                  | Coq_node (c4, _, _, _, _)
-                                                    -> (
-                                                      match c4 with
-                                                      | Red ->
-                                                          flip_colors
-                                                            (make_black
-                                                               (rot_left t))
-                                                      | Black -> t))))
-                                      | Black -> t))
-                              | Coq_node (c2, _, _, _, _) -> (
-                                  match c2 with
-                                  | Red ->
-                                      let temp_t =
-                                        Coq_node (Black, rot_left l, k, vk, r)
-                                      in
-                                      flip_colors
-                                        (make_black (rot_right temp_t))
-                                  | Black -> (
-                                      match r with
-                                      | Coq_nil -> t
-                                      | Coq_node (c3, r2, _, _, r3) -> (
-                                          match c3 with
-                                          | Red -> (
-                                              match r2 with
-                                              | Coq_nil -> (
-                                                  match r3 with
-                                                  | Coq_nil -> t
-                                                  | Coq_node (c4, _, _, _, _)
-                                                    -> (
-                                                      match c4 with
-                                                      | Red ->
-                                                          flip_colors
-                                                            (make_black
-                                                               (rot_left t))
-                                                      | Black -> t))
-                                              | Coq_node (c4, _, _, _, _) -> (
-                                                  match c4 with
-                                                  | Red ->
-                                                      let temp_t =
-                                                        Coq_node
-                                                          ( Black,
-                                                            l,
-                                                            k,
-                                                            vk,
-                                                            rot_right r )
-                                                      in
-                                                      flip_colors
-                                                        (make_black
-                                                           (rot_left temp_t))
-                                                  | Black -> (
-                                                      match r3 with
-                                                      | Coq_nil -> t
-                                                      | Coq_node (c5, _, _, _, _)
-                                                        -> (
-                                                          match c5 with
-                                                          | Red ->
-                                                              flip_colors
-                                                                (make_black
-                                                                   (rot_left t))
-                                                          | Black -> t))))
-                                          | Black -> t))))))
-                  | Black -> (
-                      match r with
-                      | Coq_nil -> t
-                      | Coq_node (c1, r2, _, _, r3) -> (
-                          match c1 with
-                          | Red -> (
-                              match r2 with
-                              | Coq_nil -> (
-                                  match r3 with
-                                  | Coq_nil -> t
-                                  | Coq_node (c2, _, _, _, _) -> (
-                                      match c2 with
+                                        Coq_node (Red, (Coq_node (Black, l,
+                                          k, vk, b0)), y0, vy0, (Coq_node
+                                          (Black, c8, z, vz, d0)))
+                                      | Black -> Coq_node (Black, l, k, vk, r)))))
+                          | Black -> Coq_node (Black, l, k, vk, r)))))
+              | Coq_node (c2, a0, x0, vx0, b) ->
+                (match c2 with
+                 | Red ->
+                   Coq_node (Red, (Coq_node (Black, a0, x0, vx0, b)), x, vx,
+                     (Coq_node (Black, c1, k, vk, r)))
+                 | Black ->
+                   (match c1 with
+                    | Coq_nil ->
+                      (match r with
+                       | Coq_nil -> Coq_node (Black, l, k, vk, r)
+                       | Coq_node (c3, b0, y, vy, d) ->
+                         (match c3 with
+                          | Red ->
+                            (match b0 with
+                             | Coq_nil ->
+                               (match d with
+                                | Coq_nil -> Coq_node (Black, l, k, vk, r)
+                                | Coq_node (c4, c5, z, vz, d0) ->
+                                  (match c4 with
+                                   | Red ->
+                                     Coq_node (Red, (Coq_node (Black, l, k,
+                                       vk, b0)), y, vy, (Coq_node (Black, c5,
+                                       z, vz, d0)))
+                                   | Black -> Coq_node (Black, l, k, vk, r)))
+                             | Coq_node (c4, b1, y0, vy0, c5) ->
+                               (match c4 with
+                                | Red ->
+                                  Coq_node (Red, (Coq_node (Black, l, k, vk,
+                                    b1)), y0, vy0, (Coq_node (Black, c5, y,
+                                    vy, d)))
+                                | Black ->
+                                  (match d with
+                                   | Coq_nil -> Coq_node (Black, l, k, vk, r)
+                                   | Coq_node (c6, c7, z, vz, d0) ->
+                                     (match c6 with
                                       | Red ->
-                                          flip_colors (make_black (rot_left t))
-                                      | Black -> t))
-                              | Coq_node (c2, _, _, _, _) -> (
-                                  match c2 with
-                                  | Red ->
-                                      let temp_t =
-                                        Coq_node (Black, l, k, vk, rot_right r)
-                                      in
-                                      flip_colors (make_black (rot_left temp_t))
-                                  | Black -> (
-                                      match r3 with
-                                      | Coq_nil -> t
-                                      | Coq_node (c3, _, _, _, _) -> (
-                                          match c3 with
-                                          | Red ->
-                                              flip_colors
-                                                (make_black (rot_left t))
-                                          | Black -> t))))
-                          | Black -> t)))))
+                                        Coq_node (Red, (Coq_node (Black, l,
+                                          k, vk, b0)), y, vy, (Coq_node
+                                          (Black, c7, z, vz, d0)))
+                                      | Black -> Coq_node (Black, l, k, vk, r)))))
+                          | Black -> Coq_node (Black, l, k, vk, r)))
+                    | Coq_node (c3, b0, y, vy, c4) ->
+                      (match c3 with
+                       | Red ->
+                         Coq_node (Red, (Coq_node (Black, a, x, vx, b0)), y,
+                           vy, (Coq_node (Black, c4, k, vk, r)))
+                       | Black ->
+                         (match r with
+                          | Coq_nil -> Coq_node (Black, l, k, vk, r)
+                          | Coq_node (c5, b1, y0, vy0, d) ->
+                            (match c5 with
+                             | Red ->
+                               (match b1 with
+                                | Coq_nil ->
+                                  (match d with
+                                   | Coq_nil -> Coq_node (Black, l, k, vk, r)
+                                   | Coq_node (c6, c7, z, vz, d0) ->
+                                     (match c6 with
+                                      | Red ->
+                                        Coq_node (Red, (Coq_node (Black, l,
+                                          k, vk, b1)), y0, vy0, (Coq_node
+                                          (Black, c7, z, vz, d0)))
+                                      | Black -> Coq_node (Black, l, k, vk, r)))
+                                | Coq_node (c6, b2, y1, vy1, c7) ->
+                                  (match c6 with
+                                   | Red ->
+                                     Coq_node (Red, (Coq_node (Black, l, k,
+                                       vk, b2)), y1, vy1, (Coq_node (Black,
+                                       c7, y0, vy0, d)))
+                                   | Black ->
+                                     (match d with
+                                      | Coq_nil ->
+                                        Coq_node (Black, l, k, vk, r)
+                                      | Coq_node (c8, c9, z, vz, d0) ->
+                                        (match c8 with
+                                         | Red ->
+                                           Coq_node (Red, (Coq_node (Black,
+                                             l, k, vk, b1)), y0, vy0,
+                                             (Coq_node (Black, c9, z, vz,
+                                             d0)))
+                                         | Black ->
+                                           Coq_node (Black, l, k, vk, r)))))
+                             | Black -> Coq_node (Black, l, k, vk, r)))))))
+           | Black ->
+             (match r with
+              | Coq_nil -> Coq_node (Black, l, k, vk, r)
+              | Coq_node (c2, b, y, vy, d) ->
+                (match c2 with
+                 | Red ->
+                   (match b with
+                    | Coq_nil ->
+                      (match d with
+                       | Coq_nil -> Coq_node (Black, l, k, vk, r)
+                       | Coq_node (c3, c4, z, vz, d0) ->
+                         (match c3 with
+                          | Red ->
+                            Coq_node (Red, (Coq_node (Black, l, k, vk, b)),
+                              y, vy, (Coq_node (Black, c4, z, vz, d0)))
+                          | Black -> Coq_node (Black, l, k, vk, r)))
+                    | Coq_node (c3, b0, y0, vy0, c4) ->
+                      (match c3 with
+                       | Red ->
+                         Coq_node (Red, (Coq_node (Black, l, k, vk, b0)), y0,
+                           vy0, (Coq_node (Black, c4, y, vy, d)))
+                       | Black ->
+                         (match d with
+                          | Coq_nil -> Coq_node (Black, l, k, vk, r)
+                          | Coq_node (c5, c6, z, vz, d0) ->
+                            (match c5 with
+                             | Red ->
+                               Coq_node (Red, (Coq_node (Black, l, k, vk,
+                                 b)), y, vy, (Coq_node (Black, c6, z, vz,
+                                 d0)))
+                             | Black -> Coq_node (Black, l, k, vk, r)))))
+                 | Black -> Coq_node (Black, l, k, vk, r))))))
 
-    (** val insert_aux : key -> 'a1 -> 'a1 rbtree -> 'a1 rbtree **)
+  (** val insert_aux : key -> 'a1 -> 'a1 rbtree -> 'a1 rbtree **)
 
-    let rec insert_aux x vx = function
-      | Coq_nil -> Coq_node (Red, Coq_nil, x, vx, Coq_nil)
-      | Coq_node (c, a, y, vy, b) ->
-          if x < y then balance (Coq_node (c, insert_aux x vx a, y, vy, b))
-          else if y < x then balance (Coq_node (c, a, y, vy, insert_aux x vx b))
-          else Coq_node (c, a, x, vx, b)
-  end
+  let rec insert_aux x vx = function
+  | Coq_nil -> Coq_node (Red, Coq_nil, x, vx, Coq_nil)
+  | Coq_node (c, a, y, vy, b) ->
+    if ( < ) x y
+    then balance (Coq_node (c, (insert_aux x vx a), y, vy, b))
+    else if ( < ) y x
+         then balance (Coq_node (c, a, y, vy, (insert_aux x vx b)))
+         else Coq_node (c, a, x, vx, b)
 
   (** val insert : key -> 'a1 -> 'a1 rbtree -> 'a1 rbtree **)
 
   let insert x vx t =
-    BalanceDetails.make_black (BalanceDetails.insert_aux x vx t)
+    make_black (insert_aux x vx t)
 
-  module UnionDetails = struct
-    (** val black_height : 'a1 rbtree -> int **)
+  (** val black_height : 'a1 rbtree -> int **)
 
-    let rec black_height = function
-      | Coq_nil -> 0
-      | Coq_node (c, l, _, _, _) -> (
-          match c with
-          | Red -> black_height l
-          | Black -> add (black_height l) (Stdlib.Int.succ 0))
+  let rec black_height = function
+  | Coq_nil -> 0
+  | Coq_node (c, l, _, _, _) ->
+    (match c with
+     | Red -> black_height l
+     | Black -> add (black_height l) (Stdlib.Int.succ 0))
 
-    (** val join_right : key -> 'a1 -> 'a1 rbtree -> 'a1 rbtree -> 'a1 rbtree **)
+  (** val join_right :
+      key -> 'a1 -> 'a1 rbtree -> 'a1 rbtree -> 'a1 rbtree **)
 
-    let rec join_right k vk l r =
-      let equal_h = black_height l = black_height r in
-      match l with
-      | Coq_nil -> insert k vk r
-      | Coq_node (c, ll, x, vx, lr) -> (
-          match c with
-          | Red -> Coq_node (Red, ll, x, vx, join_right k vk lr r)
-          | Black ->
-              if equal_h then Coq_node (Red, l, k, vk, r)
-              else
-                let t' = Coq_node (Black, ll, x, vx, join_right k vk lr r) in
-                BalanceDetails.balance t')
+  let rec join_right k vk l r =
+    let equal_h = (=) (black_height l) (black_height r) in
+    (match l with
+     | Coq_nil -> insert k vk r
+     | Coq_node (c, ll, x, vx, lr) ->
+       (match c with
+        | Red -> Coq_node (Red, ll, x, vx, (join_right k vk lr r))
+        | Black ->
+          if equal_h
+          then Coq_node (Red, l, k, vk, r)
+          else let t' = Coq_node (Black, ll, x, vx, (join_right k vk lr r)) in
+               balance t'))
 
-    (** val join_left : key -> 'a1 -> 'a1 rbtree -> 'a1 rbtree -> 'a1 rbtree **)
+  (** val join_left : key -> 'a1 -> 'a1 rbtree -> 'a1 rbtree -> 'a1 rbtree **)
 
-    let rec join_left k vk l r =
-      let equal_h = black_height l = black_height r in
-      match r with
-      | Coq_nil -> insert k vk l
-      | Coq_node (c, rl, x, vx, rr) -> (
-          match c with
-          | Red -> Coq_node (Red, join_left k vk l rl, x, vx, rr)
-          | Black ->
-              if equal_h then Coq_node (Red, l, k, vk, r)
-              else
-                let t' = Coq_node (Black, join_left k vk l rl, x, vx, rr) in
-                BalanceDetails.balance t')
+  let rec join_left k vk l r =
+    let equal_h = (=) (black_height l) (black_height r) in
+    (match r with
+     | Coq_nil -> insert k vk l
+     | Coq_node (c, rl, x, vx, rr) ->
+       (match c with
+        | Red -> Coq_node (Red, (join_left k vk l rl), x, vx, rr)
+        | Black ->
+          if equal_h
+          then Coq_node (Red, l, k, vk, r)
+          else let t' = Coq_node (Black, (join_left k vk l rl), x, vx, rr) in
+               balance t'))
 
-    (** val join : key -> 'a1 -> 'a1 rbtree -> 'a1 rbtree -> 'a1 rbtree **)
+  (** val join : key -> 'a1 -> 'a1 rbtree -> 'a1 rbtree -> 'a1 rbtree **)
 
-    let join k vk l r =
-      if Nat.ltb (black_height r) (black_height l) then
-        let t' = join_right k vk l r in
-        match t' with
-        | Coq_nil -> t'
-        | Coq_node (c, _, _, _, r1) -> (
-            match c with
-            | Red -> (
-                match r1 with
+  let join k vk l r =
+    if Nat.ltb (black_height r) (black_height l)
+    then let t' = join_right k vk l r in
+         (match t' with
+          | Coq_nil -> t'
+          | Coq_node (c, _, _, _, r1) ->
+            (match c with
+             | Red ->
+               (match r1 with
                 | Coq_nil -> t'
-                | Coq_node (c0, _, _, _, _) -> (
-                    match c0 with
-                    | Red -> BalanceDetails.make_black t'
-                    | Black -> t'))
-            | Black -> t')
-      else if Nat.ltb (black_height l) (black_height r) then
-        let t' = join_left k vk l r in
-        match t' with
-        | Coq_nil -> t'
-        | Coq_node (c, r0, _, _, _) -> (
-            match c with
-            | Red -> (
-                match r0 with
-                | Coq_nil -> t'
-                | Coq_node (c0, _, _, _, _) -> (
-                    match c0 with
-                    | Red -> BalanceDetails.make_black t'
-                    | Black -> t'))
-            | Black -> t')
-      else
-        match l with
-        | Coq_nil -> Coq_node (Black, l, k, vk, r)
-        | Coq_node (c, _, _, _, _) -> (
-            match c with
-            | Red -> Coq_node (Black, l, k, vk, r)
-            | Black -> (
-                match r with
-                | Coq_nil -> Coq_node (Black, l, k, vk, r)
-                | Coq_node (c0, _, _, _, _) -> (
-                    match c0 with
-                    | Red -> Coq_node (Black, l, k, vk, r)
-                    | Black -> Coq_node (Red, l, k, vk, r))))
+                | Coq_node (c0, _, _, _, _) ->
+                  (match c0 with
+                   | Red -> make_black t'
+                   | Black -> t'))
+             | Black -> t'))
+    else if Nat.ltb (black_height l) (black_height r)
+         then let t' = join_left k vk l r in
+              (match t' with
+               | Coq_nil -> t'
+               | Coq_node (c, r0, _, _, _) ->
+                 (match c with
+                  | Red ->
+                    (match r0 with
+                     | Coq_nil -> t'
+                     | Coq_node (c0, _, _, _, _) ->
+                       (match c0 with
+                        | Red -> make_black t'
+                        | Black -> t'))
+                  | Black -> t'))
+         else (match l with
+               | Coq_nil -> Coq_node (Black, l, k, vk, r)
+               | Coq_node (c, _, _, _, _) ->
+                 (match c with
+                  | Red -> Coq_node (Black, l, k, vk, r)
+                  | Black ->
+                    (match r with
+                     | Coq_nil -> Coq_node (Black, l, k, vk, r)
+                     | Coq_node (c0, _, _, _, _) ->
+                       (match c0 with
+                        | Red -> Coq_node (Black, l, k, vk, r)
+                        | Black -> Coq_node (Red, l, k, vk, r)))))
 
-    (** val split : key -> 'a1 rbtree -> ('a1 rbtree * bool) * 'a1 rbtree **)
+  (** val split : key -> 'a1 rbtree -> ('a1 rbtree * bool) * 'a1 rbtree **)
 
-    let rec split k = function
-      | Coq_nil -> ((Coq_nil, false), Coq_nil)
-      | Coq_node (_, l, tk, vtk, r) ->
-          if k < tk then
-            let p, r' = split k l in
-            (p, join tk vtk r' r)
-          else if tk < k then
-            let p, r' = split k r in
-            let l', b = p in
-            ((join tk vtk l l', b), r')
-          else ((l, true), r)
-  end
+  let rec split k = function
+  | Coq_nil -> (Coq_nil , false) , Coq_nil
+  | Coq_node (_, l, tk, vtk, r) ->
+    if ( < ) k tk
+    then let p , r' = split k l in p , (join tk vtk r' r)
+    else if ( < ) tk k
+         then let p , r' = split k r in
+              let l' , b = p in ((join tk vtk l l') , b) , r'
+         else (l , true) , r
 
   (** val union : 'a1 rbtree -> 'a1 rbtree -> 'a1 rbtree **)
 
   let rec union t1 t2 =
     match t1 with
-    | Coq_nil -> (
-        match t2 with Coq_nil -> Coq_nil | Coq_node (_, _, _, _, _) -> t2)
-    | Coq_node (_, _, _, _, _) -> (
-        match t2 with
-        | Coq_nil -> t1
-        | Coq_node (_, l2, k2, vk2, r2) ->
-            let p, r1 = UnionDetails.split k2 t1 in
-            let l1, _ = p in
-            let tl = union l1 l2 in
-            let tr = union r1 r2 in
-            UnionDetails.join k2 vk2 tl tr)
+    | Coq_nil ->
+      (match t2 with
+       | Coq_nil -> Coq_nil
+       | Coq_node (_, _, _, _, _) -> t2)
+    | Coq_node (_, _, _, _, _) ->
+      (match t2 with
+       | Coq_nil -> t1
+       | Coq_node (_, l2, k2, vk2, r2) ->
+         let p , r1 = split k2 t1 in
+         let l1 , _ = p in
+         let tl = union l1 l2 in let tr = union r1 r2 in join k2 vk2 tl tr)
 
   (** val delete : key -> 'a1 rbtree -> 'a1 rbtree * bool **)
 
   let delete k t =
-    let p, r = UnionDetails.split k t in
-    let l, b = p in
-    if b then (union l r, true) else (t, false)
+    let p , r = split k t in
+    let l , b = p in if b then (union l r) , true else t , false
 
   (** val size : 'a1 rbtree -> int **)
 
   let rec size = function
-    | Coq_nil -> 0
-    | Coq_node (_, l, _, _, r) ->
-        add (add (size l) (Stdlib.Int.succ 0)) (size r)
+  | Coq_nil -> 0
+  | Coq_node (_, l, _, _, r) ->
+    add (add (size l) (Stdlib.Int.succ 0)) (size r)
 
-  module FoldDetails = struct
-    (** val elements_aux : 'a1 rbtree -> (key * 'a1) list -> (key * 'a1) list **)
+  (** val elements_aux :
+      'a1 rbtree -> (key * 'a1) list -> (key * 'a1) list **)
 
-    let rec elements_aux t acc =
-      match t with
-      | Coq_nil -> acc
-      | Coq_node (_, l, k, v, r) -> elements_aux l ((k, v) :: elements_aux r acc)
+  let rec elements_aux t acc =
+    match t with
+    | Coq_nil -> acc
+    | Coq_node (_, l, k, v, r) ->
+      elements_aux l ((k , v)::(elements_aux r acc))
 
-    (** val next : key -> 'a1 rbtree -> (key * 'a1) option **)
+  (** val next : key -> 'a1 rbtree -> (key * 'a1) option **)
 
-    let rec next k = function
-      | Coq_nil -> None
-      | Coq_node (_, l, nk, vnk, r) ->
-          if k < nk then
-            match next k l with Some p -> Some p | None -> Some (nk, vnk)
-          else if nk < k then next k r
-          else min r
+  let rec next k = function
+  | Coq_nil -> None
+  | Coq_node (_, l, nk, vnk, r) ->
+    if ( < ) k nk
+    then (match next k l with
+          | Some p -> Some p
+          | None -> Some (nk , vnk))
+    else if ( < ) nk k then next k r else min r
 
-    (** val foldr_aux : 'a2 -> ((key * 'a1) -> 'a2 -> 'a2) -> key -> 'a1 rbtree
-        -> int -> 'a2 **)
+  (** val foldr_aux :
+      'a2 -> ((key * 'a1) -> 'a2 -> 'a2) -> key -> 'a1 rbtree -> int -> 'a2 **)
 
-    let rec foldr_aux init f k t fuel =
-      match next k t with
-      | Some p ->
-          let nk, vnk = p in
-          (fun fO fS n -> if n = 0 then fO () else fS (n - 1))
-            (fun _ -> init)
-            (fun pfuel -> f (nk, vnk) (foldr_aux init f nk t pfuel))
-            fuel
-      | None -> init
-  end
+  let rec foldr_aux init f k t fuel =
+    match next k t with
+    | Some p ->
+      let nk , vnk = p in
+      ((fun fO fS n -> if n=0 then fO () else fS (n-1))
+         (fun _ -> init)
+         (fun pfuel -> f (nk , vnk) (foldr_aux init f nk t pfuel))
+         fuel)
+    | None -> init
 
   (** val foldr : 'a2 -> ((key * 'a1) -> 'a2 -> 'a2) -> 'a1 rbtree -> 'a2 **)
 
   let foldr init f t =
     match min t with
     | Some p ->
-        let fst, fstv = p in
-        let fuel = size t in
-        f (fst, fstv) (FoldDetails.foldr_aux init f fst t fuel)
+      let fst , fstv = p in
+      let fuel = size t in f (fst , fstv) (foldr_aux init f fst t fuel)
     | None -> init
 
   (** val elements : 'a1 rbtree -> (key * 'a1) list **)
 
-  let elements t = FoldDetails.elements_aux t []
+  let elements t =
+    elements_aux t []
 
-  module EqbDetails = struct
-    (** val eqb_aux : key -> 'a1 rbtree -> 'a1 rbtree -> int -> bool **)
+  (** val eqb_aux : key -> 'a1 rbtree -> 'a1 rbtree -> int -> bool **)
 
-    let rec eqb_aux k t1 t2 fuel =
-      match FoldDetails.next k t1 with
-      | Some p -> (
-          let nk1, _ = p in
-          match FoldDetails.next k t2 with
-          | Some p0 ->
-              let nk2, _ = p0 in
-              (fun fO fS n -> if n = 0 then fO () else fS (n - 1))
-                (fun _ -> false)
-                (fun pfuel ->
-                  if nk1 == nk2 then eqb_aux nk1 t1 t2 pfuel else false)
-                fuel
-          | None -> false)
-      | None -> (
-          match FoldDetails.next k t2 with
-          | Some _ -> false
-          | None ->
-              (fun fO fS n -> if n = 0 then fO () else fS (n - 1))
-                (fun _ -> true)
-                (fun _ -> false)
-                fuel)
-  end
+  let rec eqb_aux k t1 t2 fuel =
+    match next k t1 with
+    | Some p ->
+      let nk1 , _ = p in
+      (match next k t2 with
+       | Some p0 ->
+         let nk2 , _ = p0 in
+         ((fun fO fS n -> if n=0 then fO () else fS (n-1))
+            (fun _ -> false)
+            (fun pfuel ->
+            if ( == ) nk1 nk2 then eqb_aux nk1 t1 t2 pfuel else false)
+            fuel)
+       | None -> false)
+    | None ->
+      (match next k t2 with
+       | Some _ -> false
+       | None ->
+         ((fun fO fS n -> if n=0 then fO () else fS (n-1))
+            (fun _ -> true)
+            (fun _ -> false)
+            fuel))
 
   (** val rbtree_eqb : 'a1 rbtree -> 'a1 rbtree -> bool **)
 
   let rbtree_eqb t1 t2 =
-    match min t1 with
-    | Some p -> (
-        let k1, _ = p in
-        match min t2 with
+    let fuel = size t1 in
+    (match min t1 with
+     | Some p ->
+       let k1 , _ = p in
+       (match min t2 with
         | Some _ ->
-            let fuel = size t1 in
-            EqbDetails.eqb_aux k1 t1 t2 (sub fuel (Stdlib.Int.succ 0))
+          ((fun fO fS n -> if n=0 then fO () else fS (n-1))
+             (fun _ -> false)
+             (fun pfuel -> eqb_aux k1 t1 t2 pfuel)
+             fuel)
         | None -> false)
-    | None -> ( match min t2 with Some _ -> false | None -> true)
-end
+     | None ->
+       (match min t2 with
+        | Some _ -> false
+        | None ->
+          ((fun fO fS n -> if n=0 then fO () else fS (n-1))
+             (fun _ -> true)
+             (fun _ -> false)
+             fuel)))
+ end
