lab-2-data-structures/Red_black_tree_proofs.v
@@ -1,0 +1,120 @@
+Require Import DataStructures.Int.
+Require Import DataStructures.Red_black_tree.
+Import Red_black_tree.
+Require Import Lia.
+
+
+Require Import ZArith.
+Open Scope Z_scope.
+
+Module Red_black_tree_proofs.
+
+Module Monoid.
+
+Lemma neutral_union_r: forall (V: Type) (t: rbtree V),
+ (union t nil) = t.
+Proof.
+  intros.
+  unfold union.
+  destruct t.
+  all: reflexivity.
+Qed.
+
+Lemma neutral_union_l: forall (V: Type) (t: rbtree V),
+ (union nil t) = t.
+Proof.
+  intros.
+  unfold union.
+  destruct t.
+  all: reflexivity.
+Qed.
+
+Lemma union_assoc: forall (V: Type) (a b c: rbtree V),
+ (union a (union b c)) = (union (union a b) c).
+ Proof.
+  intros.
+  remember a as a'.
+  induction a'.
+  - rewrite neutral_union_l.
+    rewrite neutral_union_l.
+    reflexivity.
+  - remember b as b'. destruct b'.
+    +  auto. rewrite neutral_union_l. reflexivity.
+    + remember c as c'. destruct c'.
+      -- auto. rewrite neutral_union_r. rewrite neutral_union_r. reflexivity.
+      -- auto. 
+          rewrite -> Heqc'. rewrite -> Heqb'. rewrite -> Heqa'.
+          rewrite -> Heqc' in IHa'1. rewrite -> Heqc' in IHa'2.   
+          rewrite -> Heqb' in IHa'1. rewrite -> Heqb' in IHa'2. 
+          
+          simpl.
+
+End Monoid.
+
+
+Fixpoint ForallT {V : Type} (P: int -> V -> Prop) (t : rbtree V) : Prop :=
+  match t with
+  | nil => True
+  | node c l k v r => P k v /\ ForallT P l /\ ForallT P r
+  end.
+
+Inductive BST {V : Type} : rbtree V -> Prop :=
+| ST_nil : BST nil
+| ST_node : forall (c : color) (l : rbtree V) (k : key) (v : V) (r : rbtree V),
+    ForallT (fun k' _ => (Int.mk_z k') < (Int.mk_z k)) l ->
+    ForallT (fun k' _ => (Int.mk_z k') > (Int.mk_z k)) r ->
+    BST l ->
+    BST r ->
+    BST (node c l k v r).
+
+
+Lemma nil_BST : forall (V : Type), BST (@mk_nil V).
+Proof.
+  unfold mk_nil. constructor.
+Qed.
+
+Theorem balance_BST: forall (V: Type) (t: rbtree V),
+  BST t -> BST (balance t).
+Proof.
+  intros. 
+  unfold balance.
+    repeat match goal with
+  | |- BST (match ?t with nil => _ | node _ _ _ _ _ => _ end) => destruct t
+  | |- BST (match ?c with | Red => _ | Black => _ end) => destruct c
+  | |- BST _ => constructor
+    end; auto; try lia.
+  - inversion H. auto.
+  Admitted.
+
+Lemma nilP: forall (V : Type) (P : key -> V -> Prop),
+    ForallT P nil.
+Proof.
+  intros.
+  unfold ForallT.
+  reflexivity.
+Qed.
+
+(* Lemma balanceP : forall (V : Type) (P : key -> V -> Prop) 
+        (c : color) (l r : rbtree V)
+                   (k : key) (v : V),
+    ForallT P l ->
+    ForallT P r ->
+    P k v ->
+    ForallT P (balance (node c l k v r)).
+Proof.
+  intros. 
+  unfold balance.
+   unfold balance.
+  repeat match goal with
+  | |- ForallT P (match ?t with nil => _ | node _ _ _ _ _ => _ end) => destruct t
+  | |- ForallT P (match ?c with | Red => _ | Black => _ end) => destruct c
+  | H: ForallT P (node _ _ _ _ _) |- _ => destruct H; auto
+  | |- ForallT P (node _ _ _ _ _) /\ ForallT P (node _ _ _ _ _) => split
+  | H: ForallT P _ /\ ForallT P _ |- _ => repeat destruct H; auto
+  end; auto.
+
+  Qed. *)
+
+  
+
+End Red_black_tree_proofs.
